\subsection{Control Input Design}
Let, the total control input be the sum of the following inputs:
\begin{align*}
    u &= u_a + u_s \qquad u_s = u_{s_1} + u_{s_2}
\end{align*}
\subsubsection{Model compensation input design with parameter adaption ($u_a$)}
Let, From eqn.~\ref{eqn::error_dyn}, we chose $u_a$ such that it compensates for
the error dynamics, i.e.,
\begin{align*}
    u_a &= - \pmb \phi^T  \hat{\pmb{\theta}} \\
    \text{where, } \qquad &\\
    \dot{\hat{\pmb{\theta}}} &= Proj_{\hat{\pmb{\theta}}}\lr{\Gamma \pmb \phi s}\\
\end{align*}
Where $\Gamma$ is a positive definite, diagonal adaption rate matrix.

We define, \itbf{Discontinuous projection mapping} $Proj()$ for a vector as follows:
\begin{align*}
    Proj_{\hat{\pmb\theta}} (\bullet) &= \bm{Proj_{\hat \theta_1}(\bullet_1), &
                                        Proj_{\hat \theta_2}(\bullet_2), &
                                        \hdots, &
                                        Proj_{\hat \theta_n}(\bullet_n)}\\
    Proj_{\hat \theta_i}(\bullet_i) &= \begin{cases}
        0 & \text{if } \begin{cases}
                        \hat \theta_i &= \hat \theta_{i_{min}} \text{  and  } \bullet_i < 0\\
                        \hat \theta_i &= \hat \theta_{i_{max}} \text{  and  } \bullet_i > 0\\
                       \end{cases}\\
        \bullet_i & \text{otherwise}
    \end{cases}
\end{align*}
The above mapping has the following properties:
\begin{itemize}
    \item[$P_1$:] $\quad \hat{\pmb \theta} \in \bar \Omega_{\theta}=\{\hat{\pmb \theta} : \theta_{i_{min}} \leq \hat \theta_i \leq \theta_{i_{max}} \; \forall i\} \; \forall t$

    \item[$P_2$:] $\quad \tilde{\pmb{\theta}} \left[ \Gamma^{-1}
    Proj_{\hat{\pmb\theta}} \lr{\Gamma \pmb \phi s} - \phi s \right] \leq 0 \:
    \forall t \qquad [\tilde{\pmb{\theta}} = \hat{\pmb\theta} - \pmb \theta]$
\end{itemize}

\subsubsection{Robust feedback control input design}
Substituting $u_a$ in eqn.~\ref{eqn::error_dyn}:
\begin{align*}
    \theta_1 \dot s &= -\pmb \phi^T \hat{\pmb \theta} + \pmb \phi^T \pmb \theta + \Delta + u_{s_1} + u_{s_2}\\
    \text{Let,  } u_{s_1} &= -k_p s & & [\text{Proportional Feedback}]\\
    \text{and  } \tilde{\pmb\theta} &= \hat{\pmb \theta} - \pmb \theta\\
    \implies \theta_1 \dot s + k_p s &= u_{s_2} - \pmb \phi^T \tilde{\pmb \theta} + \Delta\\
\end{align*}
Let $- \pmb \phi^T \tilde{\pmb \theta} + \Delta$ be bounded by $h(\omega, t)$,
i.e.,
\begin{align*}
    h(\omega, t) &\geq   - \pmb \phi^T \tilde{\pmb \theta} + \Delta  \quad \forall t\\
    \implies h &= \abs{\pmb \phi^T} \tilde{\pmb \theta}_M + \abs{\Delta}\\
               &= \abs{\pmb \phi^T} \tilde{\pmb \theta}_M + \Delta_M \qquad
                \tilde{\pmb \theta}_M = \pmb \theta_{max} - \pmb \theta_{min}\\
\end{align*}

Use sliding mode control law for $u_{s_2}$:
\begin{align*}
    u_{s_2} &= S(h \sign(s))\\
    \text{Where,  } \qquad &\\
    S(h \sign(s)) &= h \sat \lr{ \frac{h}{4 \varepsilon} s} &[\text{Smoothing function}]\\
    \sat (x) &= \begin{cases}
        x  & \text{if  } \abs{x} \leq   1\\
        \sign(x) &  \text{otherwise}
    \end{cases}
\end{align*}
The above defined smoothing function, $S(.)$, has the following properties:

\begin{itemize}
\item[$P_3$:] $s S(h \sign(s)) = s h \sat \lr{\frac{h}{4 \varepsilon} s} \geq
0 \qquad $ $\because$ $s$ and $\sat \lr{\frac{h}{4 \varepsilon} s}$ have the
same sign.

\item[$P_4$:] $s \left[h \sign(s) - S(h\sign(s)) \right]$ is bounded.
\begin{align*}
    s \left[h \sign(s) - S(h\sign(s)) \right] &= s \left[h \sign(s) - h \sat \lr{\frac{h}{4 \varepsilon} s} \right]
\end{align*}
\begin{enumerate}
\item Outside the boundary layer, i.e., $\lr{\abs{s} > \frac{4 \varepsilon}{h}
}$:
\begin{align*}
    sh \sign(s) - s h \sat \lr{\frac{h}{4 \varepsilon} s} &= h \abs{s} - h\abs{s} = 0
\end{align*}

\item Inside the boundary layer, i.e., $\lr{\abs{s} < \frac{4 \varepsilon}{h}}$
\begin{align*}
    sh \sign(s) - s h \sat \lr{\frac{h}{4 \varepsilon} s} &= h \abs{s} - \frac{h^2}{4 \varepsilon} s^2\\
    &= \varepsilon - \left[ \frac{1}{2 \sqrt{\varepsilon}} h \abs{s} - \sqrt{\varepsilon} \right]^2\\
    &\leq \varepsilon\\
    s \left[h \sign(s) - S(h\sign(s)) \right] &\leq \varepsilon
\end{align*}
\end{enumerate}
\end{itemize}

Thus, we have the DARC control law:
\begin{align*}
    u &= u_a + u_{s_1} + u_{s_2}\\
    u_a &= - \pmb \phi^T \hat{\pmb \theta} \qquad  \qquad
    \dot{\hat{\pmb \theta}} = Proj_{\hat{\pmb \theta}} \lr{\Gamma \pmb \phi s}\\
    u_{s_1} &= -k_p s\\
    u_{s_2} &= S(h \sign(s)) = h \sat \lr{\frac{h}{4 \varepsilon} s}
\end{align*}
