\subsection{Stability and tracking performance}
\subsubsection{Case 1: $\Delta = 0$}
When $\Delta = 0$ consider the following Lyapunov function:
\begin{align*}
    V &= \frac{1}{2} \theta_1 s^2 + \frac{1}{2} \tilde{\pmb \theta}^T \Gamma^{-1} \tilde{\pmb \theta}\\
    %===
    \dot V &= s \theta_1 + \tilde{\pmb \theta} \Gamma^{-1} \underbrace{\dot{\tilde{\pmb \theta}}}_{=\dot{\hat{\pmb \theta}}}\\
    %===
    &= s \lr{ -k_p s + \underbrace{u_{s_2}}_{=0} - \tilde{\pmb \theta} \pmb \phi } + \tilde{\pmb \theta} \Gamma^{-1} Proj_{\hat{\pmb \theta}} \lr{\Gamma \Phi s}\\
    %===
    &= -k_p s^2 + \underbrace{\tilde{\pmb \theta}^T \lr{-\pmb \phi s + \Gamma^{-1}Proj_{\hat{\pmb \theta}} \lr{\Gamma \Phi s}}}_{\leq 0} \qquad [P_2]\\
    %===
    \implies \dot V \leq -k_p s^2 \leq 0
\end{align*}
Thus,
\begin{itemize}
    \item $\dot V$ is negative semi-definite.
    \item $V$ has a lower bound $(\geq 0)$.
    \item $\dot V$ is uniform continuous $(\ddot V \leq -k_p s \dot s)$.
    \item $\therefore$ For a bounded $\omega_d$, $s \in L_\infty$, $\tilde{\pmb
    \theta} \in L_{\infty}$ and $\dot s \in L_\infty$, $\ddot V \in L_\infty$.
\end{itemize}

Hence, the parameter estimates and tracking errors are bounded and the system is
stable.

\bigskip

Also, since $V$ is non-decreasing and positive definite,
\begin{align*}
    V(0) - V(t) &\leq V(0) \quad
    \implies -\int_0^t V d \tau \leq V(0)\\
    \implies \int_0^t k_p s^2 d \tau &\leq V(0)\\
    \implies \sqrt{\int_0^t \norm{s}^2 d \tau } &\leq \sqrt{\frac{2 V(0)}{k_p}} \leq \infty\\
    \therefore s &\in L_2
\end{align*}
From Barbalat's lemma, we have,
\begin{align*}
    \dot V \rightarrow 0 \quad s \rightarrow 0 \quad \text{as} \quad t \rightarrow 0
\end{align*}
Thus the parameter estimates are bounded, and the tracking error asymptotically
goes to zero as  $t \rightarrow 0$.


\subsubsection{Case 2: $\Delta \neq 0$}
Consider the following Lyapunov function:
\begin{align*}
    V &= \frac{1}{2} \theta_1 s^2\\
    \implies \dot V &= s \theta_1 \dot s = s \lr{-k_p s + u_{s_2} - \pmb \phi^T \tilde{\pmb \theta} + \Delta }\\
    %===
    &= -k_p s^2 + s \lr{-\pmb \phi^T \tilde{\pmb \theta} + \Delta - S(h \sign(s))}\\
    &\leq -k_p s^2 + s \lr{\abs{\pmb \phi^T} \tilde{\pmb \theta}_M + \abs{\Delta} - S(h \sign(s))}
    = -k_p s^2 + \underbrace{s \lr{h\sign(s)- S(h \sign(s))}}_{\leq \varepsilon} \quad [\because P_4] \\
    \implies \dot V &\leq -k_p s^2 + \varepsilon = - \frac{2 k_p}{\theta_1} V + \varepsilon
\end{align*}
By applying comparison lemma, the upper bound can be found from the forced
response of the following ODE:
\begin{align*}
    \dot V + \frac{2 k_p}{\theta_1} V &= \varepsilon\\
    \implies sV - V(0) + \frac{2 k_p}{\theta_1} V &= \varepsilon\\
    \implies V &= \frac{V(0)}{s + \frac{2 k_p}{\theta_1}} + \frac{\varepsilon}{\frac{2 k_p}{\theta_1}}\\
    \implies V(t) &= V(0)e^{\frac{2 k_p}{\theta_1} t} + \int_0^t{e^{\frac{2 k_p}{\theta_1} (t-\tau)} \varepsilon(\tau) d\tau}\\
    \implies \frac{1}{2} \theta_1 s^2 &= \frac{1}{2} \theta_1 s(0)^2 e^{\frac{2 k_p}{\theta_1} t} + \int_0^t{e^{\frac{2 k_p}{\theta_1} (t-\tau)} \varepsilon(\tau) d\tau}\\
    %===
    \implies \abs{s(t)}^2 &= s(0)^2 e^{\frac{2 k_p}{\theta_1} t} +\frac{1}{\frac{1}{2} \theta_1 } \int_0^t{e^{\frac{2 k_p}{\theta_1} (t-\tau)} \varepsilon(\tau) d\tau}\\
    &\leq s(0)^2 e^{\frac{2 k_p}{\theta_1} t} + \frac{\varepsilon_M}{k_p} \left[1 -  e^{\frac{2 k_p}{\theta_1} t} \right]\\
    %==
\end{align*}
This the system is stable, and the transient response is bounded that
exponentially converges to $\frac{\varepsilon}{k_p}$.
